

Sheet 2

1)

a) $|\psi(t)\rangle = U(t)|\psi(0)\rangle, U(t) = e^{-iHt/\hbar}$

$$H = \frac{\hbar\omega_0}{2} \sigma_z$$

$$U(t) = e^{-i\left(\frac{\hbar\omega_0}{2} \sigma_z\right)t/\hbar} = e^{-i\frac{\omega_0 t}{2} \sigma_z}$$

$$U(t)|0\rangle = e^{-i\frac{\omega_0 t}{2}(+1)}|0\rangle = e^{-i\omega_0 t/2}|0\rangle$$

$$U(t)|1\rangle = e^{-i\frac{\omega_0 t}{2}(-1)}|1\rangle = e^{+i\omega_0 t/2}|1\rangle$$

$$|\psi(0)\rangle = \frac{1}{\sqrt{2}}(|0\rangle + i|1\rangle)$$

$$|\psi(t)\rangle = U(t)\frac{1}{\sqrt{2}}(|0\rangle + i|1\rangle) = \frac{1}{\sqrt{2}}(U(t)|0\rangle + iU(t)|1\rangle)$$

$$\Rightarrow |\psi(t)\rangle = \frac{1}{\sqrt{2}}\left(e^{-i\omega_0 t/2}|0\rangle + ie^{i\omega_0 t/2}|1\rangle\right)$$

1)

b) $X = \frac{1}{\sqrt{2}}(|0\rangle + |1\rangle)$

The Eigenvalues of Pauli matrix, σ_x , are -1 and 1 (1 and -1).

$$+1: |+\rangle_x = \frac{1}{\sqrt{2}}(|0\rangle + |1\rangle)$$

$$-1: |-\rangle_x = \frac{1}{\sqrt{2}}(|0\rangle - |1\rangle)$$

$$P(+1) = |\langle +_x | \psi(t) \rangle|^2$$

$$\langle +_x | \psi(t) \rangle = \frac{1}{2} \left(e^{-i\omega_0 t/2} + ie^{i\omega_0 t/2} \right)$$

$$P(+1) = \left| \frac{1}{2} \left(e^{-i\omega_0 t/2} + ie^{i\omega_0 t/2} \right) \right|^2$$

$$1) \quad b) \quad P(+1) = \frac{1}{4} \left(e^{-i\omega_0 t/2} \cdot e^{i\omega_0 t/2} \right) \left(e^{i\omega_0 t/2} \cdot e^{-i\omega_0 t/2} \right) \\
P(+1) = \frac{1}{4} (2 + 2 \sin(\omega_0 t)) = \frac{1}{2} (1 + \sin(\omega_0 t)) \\
-1: P(-1) = 1 - P(+1)$$

$$\boxed{P(+1) = \frac{1}{2} (1 + \sin(\omega_0 t))} \\
\boxed{P(-1) = \frac{1}{2} (1 - \sin(\omega_0 t))}$$

$$1) \quad c) \quad F(\omega_0) = \frac{1}{P(+1)} \left(\frac{\partial P(+1)}{\partial \omega_0} \right)^2 + \frac{1}{P(-1)} \left(\frac{\partial P(-1)}{\partial \omega_0} \right)^2$$

$$\frac{\partial P(+1)}{\partial \omega_0} = \frac{\partial}{\partial \omega_0} \left[\frac{1}{2} (1 + \sin(\omega_0 t)) \right] = \frac{t}{2} \cos(\omega_0 t)$$

$$\frac{\partial P(-1)}{\partial \omega_0} = \frac{\partial}{\partial \omega_0} \left[\frac{1}{2} (1 - \sin(\omega_0 t)) \right] = -\frac{t}{2} \cos(\omega_0 t)$$

$$F(\omega_0) = \frac{\left(\frac{t}{2} \cos(\omega_0 t) \right)^2}{\frac{1}{2} (1 + \sin(\omega_0 t))} + \frac{\left(-\frac{t}{2} \cos(\omega_0 t) \right)^2}{\frac{1}{2} (1 - \sin(\omega_0 t))}$$

$$F(\omega_0) = \frac{t^2 \cos^2(\omega_0 t)}{2} \left[\frac{2}{1 - \sin^2(\omega_0 t)} \right] = \frac{t^2 \cos^2(\omega_0 t)}{2}$$

$$\cdot \left[\frac{2}{\cos^2(\omega_0 t)} \right] \Rightarrow \boxed{F(\omega_0) = t^2}$$

$$1) \quad d) \quad H(t) = \frac{\hbar \omega_0}{2i} \cos(\omega_0 t) \sigma_z$$

$$U(t) = e^{-\frac{i}{\hbar} \int_0^t H(t') dt'}$$

$$\int_0^t H(t') dt' = \int_0^t \frac{\hbar \omega_0}{2} \cos(\omega_0 t') \sigma_z dt'$$

$$1) d) \int_0^t f(t') dt' = \int_0^t \frac{\hbar \omega_0}{2} \cos(\omega t') \sigma_z dt' =$$

$$\int_0^t f(t') dt' = \frac{\hbar \omega_0}{2} \sigma_z \left[\frac{\sin(\omega t')}{\omega} \right]_0^t =$$

$$\int_0^t f(t') dt' = \frac{\hbar \omega_0}{2\omega} \sin(\omega t) \sigma_z$$

$$U(t) = e^{-\frac{i}{\hbar} \left(\frac{\hbar \omega_0}{2\omega} \sin(\omega t) \sigma_z \right)}$$

$$U(t) = e^{-i \frac{\omega_0}{2\omega} \sin(\omega t) \sigma_z}$$

$$|\psi(0)\rangle = \frac{1}{\sqrt{2}} (|0\rangle + i|1\rangle)$$

$$|\psi(t)\rangle = U(t) |\psi(0)\rangle$$

$$e^{-i\phi \sigma_z} |0\rangle = e^{-i\phi} |0\rangle, e^{-i\phi \sigma_z} |1\rangle = e^{+i\phi} |1\rangle$$

$$\phi = \frac{\omega_0}{2\omega} \sin(\omega t) \Rightarrow$$

$$\Rightarrow |\psi(t)\rangle = \frac{1}{\sqrt{2}} \left(e^{-i \frac{\omega_0}{2\omega} \sin(\omega t)} |0\rangle + i e^{i \frac{\omega_0}{2\omega} \sin(\omega t)} |1\rangle \right)$$

$$1) e) F'(\omega_0) = \left(\frac{d}{d\omega_0} \left[\omega_0 \frac{\sin(\omega t)}{\omega} \right] \right)^2 = \left(\frac{\sin(\omega t)}{\omega} \right)^2$$

$$F(\omega_0) = \frac{\sin^2(\omega t)}{\omega^2}$$

Scenario 1 - Constant Field: $F(\omega_0) = t^2$ - ω_0 grow

Scenario 2 - Oscillating Field: $F'(\omega_0) = \frac{\sin^2(\omega t)}{\omega^2}$

Scenario 1 - Constant Field: $F(\omega) = \ell^2$ - ω grows without bound

Scenario 2 - Oscillating Field: $F(\omega) = \frac{\pi^2(\omega\ell)}{\omega^2}$ -
Oscillates and bounded by a maximum value of $\frac{1}{\omega^2}$

Sheet 2

1. Suppose that you want to measure a parameter ω_0 . You choose a two-level system as your quantum probe. This parameter shows up in the Hamiltonian of your probe: $H = \frac{\hbar\omega_0}{2}\sigma_z$. You initialize the probe in the state $|\psi(0)\rangle = \frac{1}{\sqrt{2}}(|0\rangle + i|1\rangle)$. Here $\sigma_z|0\rangle = |0\rangle$ and $\sigma_z|1\rangle = -|1\rangle$.
- (a) What is the state of the probe at time t ?
 - (b) Suppose that at time t , I measure the observable $X = |0\rangle\langle 1| + |1\rangle\langle 0|$. What are the possible measurement results? What are the corresponding probabilities?
 - (c) Given these probabilities, what is the Fisher information for the estimation of ω_0 ? Sketch this versus time.
 - (d) Suppose now that the Hamiltonian is $H = \frac{\hbar\omega_0}{2}\cos(\omega t)$. This happens when we have to measure an oscillating field. What is the time at time t now?
 - (e) We again perform a measurement of the observable X . What is the Fisher information now? Compare with the previous scenario and comment.